src/Std/Data/DTreeMap/Internal/Lemmas.lean
@@ -61,7 +61,10 @@ private def helperLemmaNames : Array Name :=
 
 private def queryNames : Array Name :=
   #[``isEmpty_eq_isEmpty, ``contains_eq_containsKey, ``size_eq_length,
-    ``get?_eq_getValueCast?, ``Const.get?_eq_getValue?]
+    ``get?_eq_getValueCast?, ``Const.get?_eq_getValue?,
+    ``get_eq_getValueCast, ``Const.get_eq_getValue,
+    ``get!_eq_getValueCast!, ``Const.get!_eq_getValue!,
+    ``getD_eq_getValueCastD, ``Const.getD_eq_getValueD]
 
 private def modifyMap : Std.HashMap Name Name :=
   .ofList
@@ -487,70 +490,460 @@ namespace Const
 
 variable {β : Type v} {t : Impl α β}
 
-theorem get?_empty [TransOrd α] {a : α} : get? a (empty : Impl α β) = none := by
+theorem get?_empty [TransOrd α] {a : α} : get? (empty : Impl α β) a = none := by
   simp_to_model using List.getValue?_nil
 
 theorem get?_of_isEmpty [TransOrd α] (h : t.WF) {a : α} :
-    t.isEmpty = true → get? a t = none := by
+    t.isEmpty = true → get? t a = none := by
   simp_to_model; empty
 
 theorem get?_insert [TransOrd α] (h : t.WF) {a k : α} {v : β} :
-    get? a (t.insert k v h.balanced).impl =
-      if compare k a = .eq then some v else get? a t := by
+    get? (t.insert k v h.balanced).impl a =
+      if compare k a = .eq then some v else get? t a := by
   simp_to_model [insert] using List.getValue?_insertEntry
 
 theorem get?_insert! [TransOrd α] (h : t.WF) {a k : α} {v : β} :
-    get? a (t.insert! k v) =
-      if compare k a = .eq then some v else get? a t := by
+    get? (t.insert! k v) a =
+      if compare k a = .eq then some v else get? t a := by
   simp_to_model [insert!] using List.getValue?_insertEntry
 
 theorem get?_insert_self [TransOrd α] (h : t.WF) {k : α} {v : β} :
-    get? k (t.insert k v h.balanced).impl = some v := by
+    get? (t.insert k v h.balanced).impl k = some v := by
   simp_to_model [insert] using List.getValue?_insertEntry_self
 
 theorem get?_insert!_self [TransOrd α] (h : t.WF) {k : α} {v : β} :
-    get? k (t.insert! k v) = some v := by
+    get? (t.insert! k v) k = some v := by
   simp_to_model [insert!] using List.getValue?_insertEntry_self
 
 theorem contains_eq_isSome_get? [TransOrd α] (h : t.WF) {a : α} :
-    t.contains a = (get? a t).isSome := by
+    t.contains a = (get? t a).isSome := by
   simp_to_model using List.containsKey_eq_isSome_getValue?
 
 theorem mem_iff_isSome_get? [TransOrd α] (h : t.WF) {a : α} :
-    a ∈ t ↔ (get? a t).isSome := by
+    a ∈ t ↔ (get? t a).isSome := by
   simpa [mem_iff_contains] using contains_eq_isSome_get? h
 
 theorem get?_eq_none_of_contains_eq_false [TransOrd α] (h : t.WF) {a : α} :
-    t.contains a = false → get? a t = none := by
+    t.contains a = false → get? t a = none := by
   simp_to_model using List.getValue?_eq_none.mpr
 
 theorem get?_eq_none [TransOrd α] (h : t.WF) {a : α} :
-    ¬ a ∈ t → get? a t = none := by
+    ¬ a ∈ t → get? t a = none := by
   simpa [mem_iff_contains] using get?_eq_none_of_contains_eq_false h
 
 theorem get?_erase [TransOrd α] (h : t.WF) {k a : α} :
-    get? a (t.erase k h.balanced).impl = if compare k a = .eq then none else get? a t := by
+    get? (t.erase k h.balanced).impl a = if compare k a = .eq then none else get? t a := by
   simp_to_model [erase] using List.getValue?_eraseKey
 
 theorem get?_erase! [TransOrd α] (h : t.WF) {k a : α} :
-    get? a (t.erase! k) = if compare k a = .eq then none else get? a t := by
+    get? (t.erase! k) a = if compare k a = .eq then none else get? t a := by
   simp_to_model [erase!] using List.getValue?_eraseKey
 
 theorem get?_erase_self [TransOrd α] (h : t.WF) {k : α} :
-    get? k (t.erase k h.balanced).impl = none := by
+    get? (t.erase k h.balanced).impl k = none := by
   simp_to_model [erase] using List.getValue?_eraseKey_self
 
 theorem get?_erase!_self [TransOrd α] (h : t.WF) {k : α} :
-    get? k (t.erase! k) = none := by
+    get? (t.erase! k) k = none := by
   simp_to_model [erase!] using List.getValue?_eraseKey_self
 
-theorem get?_eq_get? [LawfulEqOrd α] [TransOrd α] (h : t.WF) {a : α} : get? a t = t.get? a := by
+theorem get?_eq_get? [LawfulEqOrd α] [TransOrd α] (h : t.WF) {a : α} : get? t a = t.get? a := by
   simp_to_model using List.getValue?_eq_getValueCast?
 
 theorem get?_congr [TransOrd α] (h : t.WF) {a b : α} (hab : compare a b = .eq) :
-    get? a t = get? b t := by
+    get? t a = get? t b := by
   revert hab
   simp_to_model using List.getValue?_congr
+
+end Const
+
+theorem get_insert [TransOrd α] [LawfulEqOrd α] (h : t.WF) {k a : α} {v : β k} {h₁} :
+    (t.insert k v h.balanced).impl.get a h₁ =
+      if h₂ : compare k a = .eq then
+        cast (congrArg β (compare_eq_iff_eq.mp h₂)) v
+      else
+        t.get a (contains_of_contains_insert h h₁ h₂) := by
+  simp_to_model [insert] using List.getValueCast_insertEntry
+
+theorem get_insert! [TransOrd α] [LawfulEqOrd α] (h : t.WF) {k a : α} {v : β k} {h₁} :
+    (t.insert! k v).get a h₁ =
+      if h₂ : compare k a = .eq then
+        cast (congrArg β (compare_eq_iff_eq.mp h₂)) v
+      else
+        t.get a (contains_of_contains_insert! h h₁ h₂) := by
+  simp_to_model [insert!] using List.getValueCast_insertEntry
+
+theorem get_insert_self [TransOrd α] [LawfulEqOrd α] (h : t.WF) {k : α} {v : β k} :
+    (t.insert k v h.balanced).impl.get k (contains_insert_self h) = v := by
+  simp_to_model [insert] using List.getValueCast_insertEntry_self
+
+theorem get_insert!_self [TransOrd α] [LawfulEqOrd α] (h : t.WF) {k : α} {v : β k} :
+    (t.insert! k v).get k (contains_insert!_self h) = v := by
+  simp_to_model [insert!] using List.getValueCast_insertEntry_self
+
+@[simp]
+theorem get_erase [TransOrd α] [LawfulEqOrd α] (h : t.WF) {k a : α} {h'} :
+    (t.erase k h.balanced).impl.get a h' = t.get a (contains_of_contains_erase h h') := by
+  simp_to_model [erase] using List.getValueCast_eraseKey
+
+theorem get_erase! [TransOrd α] [LawfulEqOrd α] (h : t.WF) {k a : α} {h'} :
+    (t.erase! k).get a h' = t.get a (contains_of_contains_erase! h h') := by
+  simp_to_model [erase!] using List.getValueCast_eraseKey
+
+theorem get?_eq_some_get [TransOrd α] [LawfulEqOrd α] (h : t.WF) {a : α} {h'} : t.get? a = some (t.get a h') := by
+  simp_to_model using List.getValueCast?_eq_some_getValueCast
+
+namespace Const
+
+variable {β : Type v} {t : Impl α β} (h : t.WF)
+
+theorem get_insert [TransOrd α] (h : t.WF) {k a : α} {v : β} {h₁} :
+    get (t.insert k v h.balanced).impl a h₁ =
+      if h₂ : compare k a = .eq then v
+      else get t a (contains_of_contains_insert h h₁ h₂) := by
+  simp_to_model [insert] using List.getValue_insertEntry
+
+theorem get_insert! [TransOrd α] (h : t.WF) {k a : α} {v : β} {h₁} :
+    get (t.insert! k v) a h₁ =
+      if h₂ : compare k a = .eq then v
+      else get t a (contains_of_contains_insert! h h₁ h₂) := by
+  simp_to_model [insert!] using List.getValue_insertEntry
+
+theorem get_insert_self [TransOrd α] (h : t.WF) {k : α} {v : β} :
+    get (t.insert k v h.balanced).impl k (contains_insert_self h) = v := by
+  simp_to_model [insert] using List.getValue_insertEntry_self
+
+theorem get_insert!_self [TransOrd α] (h : t.WF) {k : α} {v : β} :
+    get (t.insert! k v) k (contains_insert!_self h) = v := by
+  simp_to_model [insert!] using List.getValue_insertEntry_self
+
+@[simp]
+theorem get_erase [TransOrd α] (h : t.WF) {k a : α} {h'} :
+    get (t.erase k h.balanced).impl a h' = get t a (contains_of_contains_erase h h') := by
+  simp_to_model [erase] using List.getValue_eraseKey
+
+theorem get_erase! [TransOrd α] (h : t.WF) {k a : α} {h'} :
+    get (t.erase! k) a h' = get t a (contains_of_contains_erase! h h') := by
+  simp_to_model [erase!] using List.getValue_eraseKey
+
+theorem get?_eq_some_get [TransOrd α] (h : t.WF) {a : α} {h} :
+    get? t a = some (get t a h) := by
+  simp_to_model using List.getValue?_eq_some_getValue
+
+theorem get_eq_get [TransOrd α] [LawfulEqOrd α] (h : t.WF) {a : α} {h} : get t a h = t.get a h := by
+  simp_to_model using List.getValue_eq_getValueCast
+
+theorem get_congr [TransOrd α] (h : t.WF) {a b : α} (hab : compare a b = .eq) {h'} :
+    get t a h' = get t b ((contains_congr h hab).symm.trans h') := by
+  revert hab h'
+  simp_to_model using List.getValue_congr
+
+end Const
+
+theorem get!_empty [TransOrd α] [LawfulEqOrd α] {a : α} [Inhabited (β a)] :
+    get! (empty : Impl α β) a = default := by
+  simp_to_model using List.getValueCast!_nil
+
+theorem get!_of_isEmpty [TransOrd α] [LawfulEqOrd α] (h : t.WF) {a : α} [Inhabited (β a)] :
+    t.isEmpty = true → t.get! a = default := by
+  simp_to_model; empty
+
+theorem get!_insert [TransOrd α] [LawfulEqOrd α] (h : t.WF) {k a : α} [Inhabited (β a)] {v : β k} :
+    (t.insert k v h.balanced).impl.get! a =
+      if h : compare k a = .eq then cast (congrArg β (compare_eq_iff_eq.mp h)) v else t.get! a := by
+  simp_to_model [insert] using List.getValueCast!_insertEntry
+
+theorem get!_insert! [TransOrd α] [LawfulEqOrd α] (h : t.WF) {k a : α} [Inhabited (β a)] {v : β k} :
+    (t.insert! k v).get! a =
+      if h : compare k a = .eq then cast (congrArg β (compare_eq_iff_eq.mp h)) v else t.get! a := by
+  simp_to_model [insert!] using List.getValueCast!_insertEntry
+
+theorem get!_insert_self [TransOrd α] [LawfulEqOrd α] (h : t.WF) {a : α} [Inhabited (β a)] {b : β a} :
+    (t.insert a b h.balanced).impl.get! a = b := by
+  simp_to_model [insert] using List.getValueCast!_insertEntry_self
+
+theorem get!_insert!_self [TransOrd α] [LawfulEqOrd α] (h : t.WF) {a : α} [Inhabited (β a)] {b : β a} :
+    (t.insert! a b).get! a = b := by
+  simp_to_model [insert!] using List.getValueCast!_insertEntry_self
+
+theorem get!_eq_default_of_contains_eq_false [TransOrd α] [LawfulEqOrd α] (h : t.WF) {a : α}
+    [Inhabited (β a)] : t.contains a = false → t.get! a = default := by
+  simp_to_model using List.getValueCast!_eq_default
+
+theorem get!_eq_default [TransOrd α] [LawfulEqOrd α] (h : t.WF) {a : α} [Inhabited (β a)] :
+    ¬ a ∈ t → t.get! a = default := by
+  simpa [mem_iff_contains] using get!_eq_default_of_contains_eq_false h
+
+theorem get!_erase [TransOrd α] [LawfulEqOrd α] (h : t.WF) {k a : α} [Inhabited (β a)] :
+    (t.erase k h.balanced).impl.get! a = if compare k a = .eq then default else t.get! a := by
+  simp_to_model [erase] using List.getValueCast!_eraseKey
+
+theorem get!_erase! [TransOrd α] [LawfulEqOrd α] (h : t.WF) {k a : α} [Inhabited (β a)] :
+    (t.erase! k).get! a = if compare k a = .eq then default else t.get! a := by
+  simp_to_model [erase!] using List.getValueCast!_eraseKey
+
+theorem get!_erase_self [TransOrd α] [LawfulEqOrd α] (h : t.WF) {k : α} [Inhabited (β k)] :
+    (t.erase k h.balanced).impl.get! k = default := by
+  simp_to_model [erase] using List.getValueCast!_eraseKey_self
+
+theorem get!_erase!_self [TransOrd α] [LawfulEqOrd α] (h : t.WF) {k : α} [Inhabited (β k)] :
+    (t.erase! k).get! k = default := by
+  simp_to_model [erase!] using List.getValueCast!_eraseKey_self
+
+theorem get?_eq_some_get!_of_contains [TransOrd α] [LawfulEqOrd α] (h : t.WF) {a : α} [Inhabited (β a)] :
+    t.contains a = true → t.get? a = some (t.get! a) := by
+  simp_to_model using List.getValueCast?_eq_some_getValueCast!
+
+theorem get?_eq_some_get! [TransOrd α] [LawfulEqOrd α] (h : t.WF) {a : α} [Inhabited (β a)] :
+    a ∈ t → t.get? a = some (t.get! a) := by
+  simpa [mem_iff_contains] using get?_eq_some_get!_of_contains h
+
+theorem get!_eq_get!_get? [TransOrd α] [LawfulEqOrd α] (h : t.WF) {a : α} [Inhabited (β a)] :
+    t.get! a = (t.get? a).get! := by
+  simp_to_model using List.getValueCast!_eq_getValueCast?
+
+theorem get_eq_get! [TransOrd α] [LawfulEqOrd α] (h : t.WF) {a : α} [Inhabited (β a)] {h} :
+    t.get a h = t.get! a := by
+  simp_to_model using List.getValueCast_eq_getValueCast!
+
+namespace Const
+
+variable {β : Type v} {t : Impl α β} (h : t.WF)
+
+theorem get!_empty [TransOrd α] [Inhabited β] {a : α} :
+    get! (empty : Impl α β) a = default := by
+  simp_to_model using List.getValue!_nil
+
+theorem get!_of_isEmpty [TransOrd α] [Inhabited β] (h : t.WF) {a : α} :
+    t.isEmpty = true → get! t a = default := by
+  simp_to_model; empty
+
+theorem get!_insert [TransOrd α] [Inhabited β] (h : t.WF) {k a : α} {v : β} :
+    get! (t.insert k v h.balanced).impl a = if compare k a = .eq then v else get! t a := by
+  simp_to_model [insert] using List.getValue!_insertEntry
+
+theorem get!_insert! [TransOrd α] [Inhabited β] (h : t.WF) {k a : α} {v : β} :
+    get! (t.insert! k v) a = if compare k a = .eq then v else get! t a := by
+  simp_to_model [insert!] using List.getValue!_insertEntry
+
+theorem get!_insert_self [TransOrd α] [Inhabited β] (h : t.WF) {k : α}
+    {v : β} : get! (t.insert k v h.balanced).impl k = v := by
+  simp_to_model [insert] using List.getValue!_insertEntry_self
+
+theorem get!_insert!_self [TransOrd α] [Inhabited β] (h : t.WF) {k : α}
+    {v : β} : get! (t.insert! k v) k = v := by
+  simp_to_model [insert!] using List.getValue!_insertEntry_self
+
+theorem get!_eq_default_of_contains_eq_false [TransOrd α] [Inhabited β] (h : t.WF) {a : α} :
+    t.contains a = false → get! t a = default := by
+  simp_to_model using List.getValue!_eq_default
+
+theorem get!_eq_default [TransOrd α] [Inhabited β] (h : t.WF) {a : α} :
+    ¬ a ∈ t → get! t a = default := by
+  simpa [mem_iff_contains] using get!_eq_default_of_contains_eq_false h
+
+theorem get!_erase [TransOrd α] [Inhabited β] (h : t.WF) {k a : α} :
+    get! (t.erase k h.balanced).impl a = if compare k a = .eq then default else get! t a := by
+  simp_to_model [erase] using List.getValue!_eraseKey
+
+theorem get!_erase! [TransOrd α] [Inhabited β] (h : t.WF) {k a : α} :
+    get! (t.erase! k) a = if compare k a = .eq then default else get! t a := by
+  simp_to_model [erase!] using List.getValue!_eraseKey
+
+theorem get!_erase_self [TransOrd α] [Inhabited β] (h : t.WF) {k : α} :
+    get! (t.erase k h.balanced).impl k = default := by
+  simp_to_model [erase] using List.getValue!_eraseKey_self
+
+theorem get!_erase!_self [TransOrd α] [Inhabited β] (h : t.WF) {k : α} :
+    get! (t.erase! k) k = default := by
+  simp_to_model [erase!] using List.getValue!_eraseKey_self
+
+theorem get?_eq_some_get!_of_contains [TransOrd α] [Inhabited β] (h : t.WF) {a : α} :
+    t.contains a = true → get? t a = some (get! t a) := by
+  simp_to_model using List.getValue?_eq_some_getValue!
+
+theorem get?_eq_some_get! [TransOrd α] [Inhabited β] (h : t.WF) {a : α} :
+    a ∈ t → get? t a = some (get! t a) := by
+  simpa [mem_iff_contains] using get?_eq_some_get!_of_contains h
+
+theorem get!_eq_get!_get? [TransOrd α] [Inhabited β] (h : t.WF) {a : α} :
+    get! t a = (get? t a).get! := by
+  simp_to_model using List.getValue!_eq_getValue?
+
+theorem get_eq_get! [TransOrd α] [Inhabited β] (h : t.WF) {a : α} {h} :
+    get t a h = get! t a := by
+  simp_to_model using List.getValue_eq_getValue!
+
+theorem get!_eq_get! [TransOrd α] [LawfulEqOrd α] [Inhabited β] (h : t.WF) {a : α} :
+    get! t a = t.get! a := by
+  simp_to_model using List.getValue!_eq_getValueCast!
+
+theorem get!_congr [TransOrd α] [Inhabited β] (h : t.WF) {a b : α}
+    (hab : compare a b = .eq) : get! t a = get! t b := by
+  revert hab
+  simp_to_model using List.getValue!_congr
+
+end Const
+
+theorem getD_empty [TransOrd α] [LawfulEqOrd α] {a : α} {fallback : β a} :
+    (empty : Impl α β).getD a fallback = fallback := by
+  simp [getD, empty]
+
+theorem getD_of_isEmpty [TransOrd α] [LawfulEqOrd α] (h : t.WF) {a : α} {fallback : β a} : t.isEmpty = true → t.getD a fallback = fallback := by
+  simp_to_model; empty
+
+theorem getD_insert [TransOrd α] [LawfulEqOrd α] (h : t.WF) {k a : α} {fallback : β a} {v : β k} :
+    (t.insert k v h.balanced).impl.getD a fallback =
+      if h : compare k a = .eq then
+        cast (congrArg β (compare_eq_iff_eq.mp h)) v
+      else t.getD a fallback := by
+  simp_to_model [insert] using List.getValueCastD_insertEntry
+
+theorem getD_insert! [TransOrd α] [LawfulEqOrd α] (h : t.WF) {k a : α} {fallback : β a} {v : β k} :
+    (t.insert! k v).getD a fallback =
+      if h : compare k a = .eq then
+        cast (congrArg β (compare_eq_iff_eq.mp h)) v
+      else t.getD a fallback := by
+  simp_to_model [insert!] using List.getValueCastD_insertEntry
+
+theorem getD_insert_self [TransOrd α] [LawfulEqOrd α] (h : t.WF) {a : α} {fallback b : β a} :
+    (t.insert a b h.balanced).impl.getD a fallback = b := by
+  simp_to_model [insert] using List.getValueCastD_insertEntry_self
+
+theorem getD_insert!_self [TransOrd α] [LawfulEqOrd α] (h : t.WF) {a : α} {fallback b : β a} :
+    (t.insert! a b).getD a fallback = b := by
+  simp_to_model [insert!] using List.getValueCastD_insertEntry_self
+
+theorem getD_eq_fallback_of_contains_eq_false [TransOrd α] [LawfulEqOrd α] (h : t.WF) {a : α} {fallback : β a} :
+    t.contains a = false → t.getD a fallback = fallback := by
+  simp_to_model using List.getValueCastD_eq_fallback
+
+theorem getD_eq_fallback [TransOrd α] [LawfulEqOrd α] (h : t.WF) {a : α} {fallback : β a} :
+    ¬ a ∈ t → t.getD a fallback = fallback := by
+  simpa [mem_iff_contains] using getD_eq_fallback_of_contains_eq_false h
+
+theorem getD_erase [TransOrd α] [LawfulEqOrd α] (h : t.WF) {k a : α} {fallback : β a} :
+    (t.erase k h.balanced).impl.getD a fallback = if compare k a = .eq then fallback else t.getD a fallback := by
+  simp_to_model [erase] using List.getValueCastD_eraseKey
+
+theorem getD_erase! [TransOrd α] [LawfulEqOrd α] (h : t.WF) {k a : α} {fallback : β a} :
+    (t.erase! k).getD a fallback = if compare k a = .eq then fallback else t.getD a fallback := by
+  simp_to_model [erase!] using List.getValueCastD_eraseKey
+
+theorem getD_erase_self [TransOrd α] [LawfulEqOrd α] (h : t.WF) {k : α} {fallback : β k} :
+    (t.erase k h.balanced).impl.getD k fallback = fallback := by
+  simp_to_model [erase] using List.getValueCastD_eraseKey_self
+
+theorem getD_erase!_self [TransOrd α] [LawfulEqOrd α] (h : t.WF) {k : α} {fallback : β k} :
+    (t.erase! k).getD k fallback = fallback := by
+  simp_to_model [erase!] using List.getValueCastD_eraseKey_self
+
+theorem get?_eq_some_getD_of_contains [TransOrd α] [LawfulEqOrd α] (h : t.WF) {a : α} {fallback : β a} :
+    t.contains a = true → t.get? a = some (t.getD a fallback) := by
+  simp_to_model using List.getValueCast?_eq_some_getValueCastD
+
+theorem get?_eq_some_getD [TransOrd α] [LawfulEqOrd α] (h : t.WF) {a : α} {fallback : β a} :
+    a ∈ t → t.get? a = some (t.getD a fallback) := by
+  simpa [mem_iff_contains] using get?_eq_some_getD_of_contains h
+
+theorem getD_eq_getD_get? [TransOrd α] [LawfulEqOrd α] (h : t.WF) {a : α} {fallback : β a} :
+    t.getD a fallback = (t.get? a).getD fallback := by
+  simp_to_model using List.getValueCastD_eq_getValueCast?
+
+theorem get_eq_getD [TransOrd α] [LawfulEqOrd α] (h : t.WF) {a : α} {fallback : β a} {h} :
+    t.get a h = t.getD a fallback := by
+  simp_to_model using List.getValueCast_eq_getValueCastD
+
+theorem get!_eq_getD_default [TransOrd α] [LawfulEqOrd α] (h : t.WF) {a : α} [Inhabited (β a)] :
+    t.get! a = t.getD a default := by
+  simp_to_model using List.getValueCast!_eq_getValueCastD_default
+
+namespace Const
+
+variable {β : Type v} {t : Impl α β} (h : t.WF)
+
+theorem getD_empty [TransOrd α] {a : α} {fallback : β} :
+    getD (empty : Impl α β) a fallback = fallback := by
+  simp_to_model using List.getValueD_nil
+
+theorem getD_of_isEmpty [TransOrd α] (h : t.WF) {a : α} {fallback : β} :
+    t.isEmpty = true → getD t a fallback = fallback := by
+  simp_to_model; empty
+
+theorem getD_insert [TransOrd α] (h : t.WF) {k a : α} {fallback v : β} :
+    getD (t.insert k v h.balanced).impl a fallback = if compare k a = .eq then v else getD t a fallback := by
+  simp_to_model [insert] using List.getValueD_insertEntry
+
+theorem getD_insert! [TransOrd α] (h : t.WF) {k a : α} {fallback v : β} :
+    getD (t.insert! k v) a fallback = if compare k a = .eq then v else getD t a fallback := by
+  simp_to_model [insert!] using List.getValueD_insertEntry
+
+theorem getD_insert_self [TransOrd α] (h : t.WF) {k : α} {fallback v : β} :
+    getD (t.insert k v h.balanced).impl k fallback = v := by
+  simp_to_model [insert] using List.getValueD_insertEntry_self
+
+theorem getD_insert!_self [TransOrd α] (h : t.WF) {k : α} {fallback v : β} :
+    getD (t.insert! k v) k fallback = v := by
+  simp_to_model [insert!] using List.getValueD_insertEntry_self
+
+theorem getD_eq_fallback_of_contains_eq_false [TransOrd α] (h : t.WF) {a : α} {fallback : β} :
+    t.contains a = false → getD t a fallback = fallback := by
+  simp_to_model using List.getValueD_eq_fallback
+
+theorem getD_eq_fallback [TransOrd α] (h : t.WF) {a : α} {fallback : β} :
+    ¬ a ∈ t → getD t a fallback = fallback := by
+  simpa [mem_iff_contains] using getD_eq_fallback_of_contains_eq_false h
+
+theorem getD_erase [TransOrd α] (h : t.WF) {k a : α} {fallback : β} :
+    getD (t.erase k h.balanced).impl a fallback = if compare k a = .eq then
+      fallback
+    else
+      getD t a fallback := by
+  simp_to_model [erase] using List.getValueD_eraseKey
+
+theorem getD_erase! [TransOrd α] (h : t.WF) {k a : α} {fallback : β} :
+    getD (t.erase! k) a fallback = if compare k a = .eq then
+      fallback
+    else
+      getD t a fallback := by
+  simp_to_model [erase!] using List.getValueD_eraseKey
+
+theorem getD_erase_self [TransOrd α] (h : t.WF) {k : α} {fallback : β} :
+    getD (t.erase k h.balanced).impl k fallback = fallback := by
+  simp_to_model [erase] using List.getValueD_eraseKey_self
+
+theorem getD_erase!_self [TransOrd α] (h : t.WF) {k : α} {fallback : β} :
+    getD (t.erase! k) k fallback = fallback := by
+  simp_to_model [erase!] using List.getValueD_eraseKey_self
+
+theorem get?_eq_some_getD_of_contains [TransOrd α] (h : t.WF) {a : α} {fallback : β} :
+    t.contains a = true → get? t a = some (getD t a fallback) := by
+  simp_to_model using List.getValue?_eq_some_getValueD
+
+theorem get?_eq_some_getD [TransOrd α] (h : t.WF) {a : α} {fallback : β} :
+    a ∈ t → get? t a = some (getD t a fallback) := by
+  simpa [mem_iff_contains] using get?_eq_some_getD_of_contains h
+
+theorem getD_eq_getD_get? [TransOrd α] (h : t.WF) {a : α} {fallback : β} :
+    getD t a fallback = (get? t a).getD fallback := by
+  simp_to_model using List.getValueD_eq_getValue?
+
+theorem get_eq_getD [TransOrd α] (h : t.WF) {a : α} {fallback : β} {h} :
+    get t a h = getD t a fallback := by
+  simp_to_model using List.getValue_eq_getValueD
+
+theorem get!_eq_getD_default [TransOrd α] [Inhabited β] (h : t.WF) {a : α} :
+    get! t a = getD t a default := by
+  simp_to_model using List.getValue!_eq_getValueD_default
+
+theorem getD_eq_getD [TransOrd α] [LawfulEqOrd α] (h : t.WF) {a : α} {fallback : β} :
+    getD t a fallback = t.getD a fallback := by
+  simp_to_model using List.getValueD_eq_getValueCastD
+
+theorem getD_congr [TransOrd α] (h : t.WF) {a b : α} {fallback : β}
+    (hab : compare a b = .eq) : getD t a fallback = getD t b fallback := by
+  revert hab
+  simp_to_model using List.getValueD_congr
 
 end Const
 
