src/Std/Data/DTreeMap/RawLemmas.lean
@@ -142,7 +142,7 @@ theorem size_insert_le [TransCmp cmp] (h : t.WF) {k : α} {v : β k} :
 
 @[simp]
 theorem erase_emptyc {k : α} :
-    (∅ : Raw α β cmp).erase k = empty :=
+    (∅ : Raw α β cmp).erase k = ∅ :=
   ext <| Impl.erase!_empty (instOrd := ⟨cmp⟩) (k := k)
 
 @[simp]
@@ -336,6 +336,309 @@ theorem get?_eq_get? [LawfulEqCmp cmp] [TransCmp cmp] (h : t.WF) {a : α} : get?
 theorem get?_congr [TransCmp cmp] (h : t.WF) {a b : α} (hab : cmp a b = .eq) :
     get? t a = get? t b :=
   Impl.Const.get?_congr h hab
+
+end Const
+
+theorem get_insert [TransCmp cmp] [LawfulEqCmp cmp] (h : t.WF) {k a : α} {v : β k} {h₁} :
+    (t.insert k v).get a h₁ =
+      if h₂ : cmp k a = .eq then
+        cast (congrArg β (compare_eq_iff_eq.mp h₂)) v
+      else
+        t.get a (mem_of_mem_insert h h₁ h₂) :=
+  Impl.get_insert! h
+
+@[simp]
+theorem get_insert_self [TransCmp cmp] [LawfulEqCmp cmp] (h : t.WF) {k : α} {v : β k} :
+    (t.insert k v).get k (mem_insert_self h) = v :=
+  Impl.get_insert!_self h
+
+@[simp]
+theorem get_erase [TransCmp cmp] [LawfulEqCmp cmp] (h : t.WF) {k a : α} {h'} :
+    (t.erase k).get a h' = t.get a (mem_of_mem_erase h h') :=
+  Impl.get_erase! h
+
+theorem get?_eq_some_get [TransCmp cmp] [LawfulEqCmp cmp] (h : t.WF) {a : α} {h'} :
+    t.get? a = some (t.get a h') :=
+  Impl.get?_eq_some_get h
+
+namespace Const
+
+variable {β : Type v} {t : Raw α β cmp}
+
+theorem get_insert [TransCmp cmp] (h : t.WF) {k a : α} {v : β} {h₁} :
+    get (t.insert k v) a h₁ =
+      if h₂ : cmp k a = .eq then v
+      else get t a (mem_of_mem_insert h h₁ h₂) :=
+  Impl.Const.get_insert! h
+
+@[simp]
+theorem get_insert_self [TransCmp cmp] (h : t.WF) {k : α} {v : β} :
+    get (t.insert k v) k (mem_insert_self h) = v :=
+  Impl.Const.get_insert!_self h
+
+@[simp]
+theorem get_erase [TransCmp cmp] (h : t.WF) {k a : α} {h'} :
+    get (t.erase k) a h' = get t a (mem_of_mem_erase h h') :=
+  Impl.Const.get_erase! h
+
+theorem get?_eq_some_get [TransCmp cmp] (h : t.WF) {a : α} {h'} :
+    get? t a = some (get t a h') :=
+  Impl.Const.get?_eq_some_get h
+
+theorem get_eq_get [TransCmp cmp] [LawfulEqCmp cmp] (h : t.WF) {a : α} {h'} :
+    get t a h' = t.get a h' :=
+  Impl.Const.get_eq_get h
+
+theorem get_congr [TransCmp cmp] (h : t.WF) {a b : α} (hab : cmp a b = .eq) {h'} :
+    get t a h' = get t b ((mem_congr h hab).mp h') :=
+  Impl.Const.get_congr h hab
+
+end Const
+
+@[simp]
+theorem get!_emptyc [TransCmp cmp] [LawfulEqCmp cmp] {a : α} [Inhabited (β a)] :
+    get! (∅ : Raw α β cmp) a = default :=
+  Impl.get!_empty
+
+theorem get!_of_isEmpty [TransCmp cmp] [LawfulEqCmp cmp] (h : t.WF) {a : α} [Inhabited (β a)] :
+    t.isEmpty = true → t.get! a = default :=
+  Impl.get!_of_isEmpty h
+
+theorem get!_insert [TransCmp cmp] [LawfulEqCmp cmp] (h : t.WF) {k a : α} [Inhabited (β a)]
+    {v : β k} : (t.insert k v).get! a =
+      if h : cmp k a = .eq then cast (congrArg β (compare_eq_iff_eq.mp h)) v else t.get! a :=
+  Impl.get!_insert! h
+
+@[simp]
+theorem get!_insert_self [TransCmp cmp] [LawfulEqCmp cmp] (h : t.WF) {a : α} [Inhabited (β a)]
+    {b : β a} : (t.insert a b).get! a = b :=
+  Impl.get!_insert!_self h
+
+theorem get!_eq_default_of_contains_eq_false [TransCmp cmp] [LawfulEqCmp cmp] (h : t.WF) {a : α}
+    [Inhabited (β a)] : t.contains a = false → t.get! a = default :=
+  Impl.get!_eq_default_of_contains_eq_false h
+
+theorem get!_eq_default [TransCmp cmp] [LawfulEqCmp cmp] (h : t.WF) {a : α} [Inhabited (β a)] :
+    ¬ a ∈ t → t.get! a = default :=
+  Impl.get!_eq_default h
+
+theorem get!_erase [TransCmp cmp] [LawfulEqCmp cmp] (h : t.WF) {k a : α} [Inhabited (β a)] :
+    (t.erase k).get! a = if cmp k a = .eq then default else t.get! a :=
+  Impl.get!_erase! h
+
+@[simp]
+theorem get!_erase_self [TransCmp cmp] [LawfulEqCmp cmp] (h : t.WF) {k : α} [Inhabited (β k)] :
+    (t.erase k).get! k = default :=
+  Impl.get!_erase!_self h
+
+theorem get?_eq_some_get!_of_contains [TransCmp cmp] [LawfulEqCmp cmp] (h : t.WF) {a : α}
+    [Inhabited (β a)] : t.contains a = true → t.get? a = some (t.get! a) :=
+  Impl.get?_eq_some_get!_of_contains h
+
+theorem get?_eq_some_get! [TransCmp cmp] [LawfulEqCmp cmp] (h : t.WF) {a : α} [Inhabited (β a)] :
+    a ∈ t → t.get? a = some (t.get! a) :=
+  Impl.get?_eq_some_get! h
+
+theorem get!_eq_get!_get? [TransCmp cmp] [LawfulEqCmp cmp] (h : t.WF) {a : α} [Inhabited (β a)] :
+    t.get! a = (t.get? a).get! :=
+  Impl.get!_eq_get!_get? h
+
+theorem get_eq_get! [TransCmp cmp] [LawfulEqCmp cmp] (h : t.WF) {a : α} [Inhabited (β a)] {h'} :
+    t.get a h' = t.get! a :=
+  Impl.get_eq_get! h
+
+namespace Const
+
+variable {β : Type v} {t : Raw α β cmp}
+
+@[simp]
+theorem get!_emptyc [TransCmp cmp] [Inhabited β] {a : α} :
+    get! (∅ : Raw α β cmp) a = default :=
+  Impl.Const.get!_empty
+
+theorem get!_of_isEmpty [TransCmp cmp] [Inhabited β] (h : t.WF) {a : α} :
+    t.isEmpty = true → get! t a = default :=
+  Impl.Const.get!_of_isEmpty h
+
+theorem get!_insert [TransCmp cmp] [Inhabited β] (h : t.WF) {k a : α} {v : β} :
+    get! (t.insert k v) a = if cmp k a = .eq then v else get! t a :=
+  Impl.Const.get!_insert! h
+
+@[simp]
+theorem get!_insert_self [TransCmp cmp] [Inhabited β] (h : t.WF) {k : α} {v : β} :
+    get! (t.insert k v) k = v :=
+  Impl.Const.get!_insert!_self h
+
+theorem get!_eq_default_of_contains_eq_false [TransCmp cmp] [Inhabited β] (h : t.WF) {a : α} :
+    t.contains a = false → get! t a = default :=
+  Impl.Const.get!_eq_default_of_contains_eq_false h
+
+theorem get!_eq_default [TransCmp cmp] [Inhabited β] (h : t.WF) {a : α} :
+    ¬ a ∈ t → get! t a = default :=
+  Impl.Const.get!_eq_default h
+
+theorem get!_erase [TransCmp cmp] [Inhabited β] (h : t.WF) {k a : α} :
+    get! (t.erase k) a = if cmp k a = .eq then default else get! t a :=
+  Impl.Const.get!_erase! h
+
+@[simp]
+theorem get!_erase_self [TransCmp cmp] [Inhabited β] (h : t.WF) {k : α} :
+    get! (t.erase k) k = default :=
+  Impl.Const.get!_erase!_self h
+
+theorem get?_eq_some_get!_of_contains [TransCmp cmp] [Inhabited β] (h : t.WF) {a : α} :
+    t.contains a = true → get? t a = some (get! t a) :=
+  Impl.Const.get?_eq_some_get! h
+
+theorem get?_eq_some_get! [TransCmp cmp] [Inhabited β] (h : t.WF) {a : α} :
+    a ∈ t → get? t a = some (get! t a) :=
+  Impl.Const.get?_eq_some_get! h
+
+theorem get!_eq_get!_get? [TransCmp cmp] [Inhabited β] (h : t.WF) {a : α} :
+    get! t a = (get? t a).get! :=
+  Impl.Const.get!_eq_get!_get? h
+
+theorem get_eq_get! [TransCmp cmp] [Inhabited β] (h : t.WF) {a : α} {h'} :
+    get t a h' = get! t a :=
+  Impl.Const.get_eq_get! h
+
+theorem get!_eq_get! [TransCmp cmp] [LawfulEqCmp cmp] [Inhabited β] (h : t.WF) {a : α} :
+    get! t a = t.get! a :=
+  Impl.Const.get!_eq_get! h
+
+theorem get!_congr [TransCmp cmp] [Inhabited β] (h : t.WF) {a b : α} (hab : cmp a b = .eq) :
+    get! t a = get! t b :=
+  Impl.Const.get!_congr h hab
+
+end Const
+
+@[simp]
+theorem getD_emptyc [TransCmp cmp] [LawfulEqCmp cmp] {a : α} {fallback : β a} :
+    (∅ : DTreeMap α β cmp).getD a fallback = fallback :=
+  Impl.getD_empty
+
+theorem getD_of_isEmpty [TransCmp cmp] [LawfulEqCmp cmp] (h : t.WF) {a : α} {fallback : β a} :
+    t.isEmpty = true → t.getD a fallback = fallback :=
+  Impl.getD_of_isEmpty h
+
+theorem getD_insert [TransCmp cmp] [LawfulEqCmp cmp] (h : t.WF) {k a : α} {fallback : β a} {v : β k} :
+    (t.insert k v).getD a fallback =
+      if h : cmp k a = .eq then
+        cast (congrArg β (compare_eq_iff_eq.mp h)) v
+      else t.getD a fallback :=
+  Impl.getD_insert! h
+
+@[simp]
+theorem getD_insert_self [TransCmp cmp] [LawfulEqCmp cmp] (h : t.WF) {a : α} {fallback b : β a} :
+    (t.insert a b).getD a fallback = b :=
+  Impl.getD_insert!_self h
+
+theorem getD_eq_fallback_of_contains_eq_false [TransCmp cmp] [LawfulEqCmp cmp] (h : t.WF) {a : α} {fallback : β a} :
+    t.contains a = false → t.getD a fallback = fallback :=
+  Impl.getD_eq_fallback_of_contains_eq_false h
+
+theorem getD_eq_fallback [TransCmp cmp] [LawfulEqCmp cmp] (h : t.WF) {a : α} {fallback : β a} :
+    ¬ a ∈ t → t.getD a fallback = fallback :=
+  Impl.getD_eq_fallback h
+
+theorem getD_erase [TransCmp cmp] [LawfulEqCmp cmp] (h : t.WF) {k a : α} {fallback : β a} :
+    (t.erase k).getD a fallback = if cmp k a = .eq then fallback else t.getD a fallback :=
+  Impl.getD_erase! h
+
+@[simp]
+theorem getD_erase_self [TransCmp cmp] [LawfulEqCmp cmp] (h : t.WF) {k : α} {fallback : β k} :
+    (t.erase k).getD k fallback = fallback :=
+  Impl.getD_erase!_self h
+
+theorem get?_eq_some_getD_of_contains [TransCmp cmp] [LawfulEqCmp cmp] (h : t.WF) {a : α}
+    {fallback : β a} : t.contains a = true → t.get? a = some (t.getD a fallback) :=
+  Impl.get?_eq_some_getD_of_contains h
+
+theorem get?_eq_some_getD [TransCmp cmp] [LawfulEqCmp cmp] (h : t.WF) {a : α} {fallback : β a} :
+    a ∈ t → t.get? a = some (t.getD a fallback) :=
+  Impl.get?_eq_some_getD h
+
+theorem getD_eq_getD_get? [TransCmp cmp] [LawfulEqCmp cmp] (h : t.WF) {a : α} {fallback : β a} :
+    t.getD a fallback = (t.get? a).getD fallback :=
+  Impl.getD_eq_getD_get? h
+
+theorem get_eq_getD [TransCmp cmp] [LawfulEqCmp cmp] (h : t.WF) {a : α} {fallback : β a} {h'} :
+    t.get a h' = t.getD a fallback :=
+  Impl.get_eq_getD h
+
+theorem get!_eq_getD_default [TransCmp cmp] [LawfulEqCmp cmp] (h : t.WF) {a : α} [Inhabited (β a)] :
+    t.get! a = t.getD a default :=
+  Impl.get!_eq_getD_default h
+
+namespace Const
+
+variable {β : Type v} {t : Raw α β cmp}
+
+@[simp]
+theorem getD_emptyc [TransCmp cmp] {a : α} {fallback : β} :
+    getD (∅ : Raw α β cmp) a fallback = fallback :=
+  Impl.Const.getD_empty
+
+theorem getD_of_isEmpty [TransCmp cmp] (h : t.WF) {a : α} {fallback : β} :
+    t.isEmpty = true → getD t a fallback = fallback :=
+  Impl.Const.getD_of_isEmpty h
+
+theorem getD_insert [TransCmp cmp] (h : t.WF) {k a : α} {fallback v : β} :
+    getD (t.insert k v) a fallback = if cmp k a = .eq then v else getD t a fallback :=
+  Impl.Const.getD_insert! h
+
+@[simp]
+theorem getD_insert_self [TransCmp cmp] (h : t.WF) {k : α} {fallback v : β} :
+    getD (t.insert k v) k fallback = v :=
+  Impl.Const.getD_insert!_self h
+
+theorem getD_eq_fallback_of_contains_eq_false [TransCmp cmp] (h : t.WF) {a : α} {fallback : β} :
+    t.contains a = false → getD t a fallback = fallback :=
+  Impl.Const.getD_eq_fallback_of_contains_eq_false h
+
+theorem getD_eq_fallback [TransCmp cmp] (h : t.WF) {a : α} {fallback : β} :
+    ¬ a ∈ t → getD t a fallback = fallback :=
+  Impl.Const.getD_eq_fallback h
+
+theorem getD_erase [TransCmp cmp] (h : t.WF) {k a : α} {fallback : β} :
+    getD (t.erase k) a fallback = if cmp k a = .eq then
+      fallback
+    else
+      getD t a fallback :=
+  Impl.Const.getD_erase! h
+
+@[simp]
+theorem getD_erase_self [TransCmp cmp] (h : t.WF) {k : α} {fallback : β} :
+    getD (t.erase k) k fallback = fallback :=
+  Impl.Const.getD_erase!_self h
+
+theorem get?_eq_some_getD_of_contains [TransCmp cmp] (h : t.WF) {a : α} {fallback : β} :
+    t.contains a = true → get? t a = some (getD t a fallback) :=
+  Impl.Const.get?_eq_some_getD_of_contains h
+
+theorem get?_eq_some_getD [TransCmp cmp] (h : t.WF) {a : α} {fallback : β} :
+    a ∈ t → get? t a = some (getD t a fallback) :=
+  Impl.Const.get?_eq_some_getD h
+
+theorem getD_eq_getD_get? [TransCmp cmp] (h : t.WF) {a : α} {fallback : β} :
+    getD t a fallback = (get? t a).getD fallback :=
+  Impl.Const.getD_eq_getD_get? h
+
+theorem get_eq_getD [TransCmp cmp] (h : t.WF) {a : α} {fallback : β} {h'} :
+    get t a h' = getD t a fallback :=
+  Impl.Const.get_eq_getD h
+
+theorem get!_eq_getD_default [TransCmp cmp] [Inhabited β] (h : t.WF) {a : α} :
+    get! t a = getD t a default :=
+  Impl.Const.get!_eq_getD_default h
+
+theorem getD_eq_getD [TransCmp cmp] [LawfulEqCmp cmp] (h : t.WF) {a : α} {fallback : β} :
+    getD t a fallback = t.getD a fallback :=
+  Impl.Const.getD_eq_getD h
+
+theorem getD_congr [TransCmp cmp] (h : t.WF) {a b : α} {fallback : β} (hab : cmp a b = .eq) :
+    getD t a fallback = getD t b fallback :=
+  Impl.Const.getD_congr h hab
 
 end Const
 
